SP1Foundations/Constraint.lean
@@ -75,11 +75,103 @@ lemma allHold_append (cs cs' : SP1ConstraintList) :
 
 end constraintList
 
-def toSailM : SP1Constraint → SailM Unit
-  | .receive (.memory shard clk addr low_limb high_limb) mult => do
+section toSailM
+
+/-- Naive version of conversion to `SailM` monad without clock sorting. -/
+def SP1ConstraintList.toSailM : SP1ConstraintList → SailM Unit
+  | (.receive (.memory _ _ addr low_limb high_limb) _) :: cs => do
       wX_bits (.Regidx <| BitVec.ofNat 5 addr.val)
-        (BitVec.ofNat 32 (low_limb + high_limb * 65536))
+        (BitVec.ofNat 32 (low_limb + high_limb * 65536));
+      SP1ConstraintList.toSailM cs
+  | _ :: cs => SP1ConstraintList.toSailM cs
   | _ => pure ()
 
-def constraints_to_SailM (cs : SP1ConstraintList) : SailM Unit :=
-  do let _ ← List.mapM toSailM cs
+example (x y : SailM Unit) : x = y := by
+  refine EStateM.ext ?_
+  sorry
+
+-- def SP1ConstraintList.toRegInit : SP1ConstraintList → SailM Unit
+--   | (.send (.memory _ _ addr low_limb high_limb) _) :: cs => do
+--       rX_bits (.Regidx <| BitVec.ofNat 5 addr.val)
+--         (BitVec.ofNat 32 (low_limb + high_limb * 65536));
+--       SP1ConstraintList.toSailM cs
+--   | _ :: cs => SP1ConstraintList.toSailM cs
+--   | _ => pure ()
+
+end toSailM
+
+section toReg
+
+-- def SP1Constraint.getClk : SP1Constraint → Option BabyBear
+--   | .send (.memory shard clk addr low_limb high_limb) mult => some clk
+--   | .receive (.memory shard clk addr low_limb high_limb) mult => some clk
+--   | _ => none
+
+-- noncomputable def SP1ConstraintList.sortClock (cs : SP1ConstraintList) : SP1ConstraintList :=
+--   cs.mergeSort (fun c1 c2 => open Classical in if c1.getClk ≤ c2.getClk then true else false)
+
+-- def toSailM' : SP1Constraint → SailM Unit
+--   | .send (.memory shard clk addr low_limb high_limb) mult => do
+--       wX_bits (.Regidx <| BitVec.ofNat 5 addr.val)
+--         (BitVec.ofNat 32 (low_limb + high_limb * 65536))
+--   | _ => pure ()
+
+-- noncomputable def constraints_to_SailM (cs : SP1ConstraintList) : SailM Unit :=
+--   do let _ ← List.mapM toSailM cs.sortClock
+
+section sailboats
+
+#check EStateM.Result
+
+lemma reg_map_ext (rmap rmap' : PreSail.SequentialState RegisterType trivialChoiceSource)
+    (hreg : rmap.regs = rmap'.regs)
+    (hcs : rmap.choiceState = rmap'.choiceState)
+    (hmem : rmap.mem = rmap'.mem)
+    (hcc : rmap.cycleCount = rmap'.cycleCount)
+    (hout : rmap.sailOutput = rmap'.sailOutput) :
+    rmap = rmap' := by
+  refine match rmap with | ⟨regs, cs, mem, (), cc, so⟩ => ?_
+  refine match rmap' with | ⟨regs', cs', mem', (), cc', so'⟩ => ?_
+  simp_all
+
+lemma wX_bits_rX_bits' (rs : regidx) (v : BitVec 32) (cont : BitVec 32 → SailM α) :
+    (do let _ ← wX_bits rs v; let v' ← rX_bits rs; cont v') =
+      (do let _ ← wX_bits rs v; cont v) := by
+  refine EStateM.ext fun reg_map => ?_
+  simp
+  rw [EStateM.run]
+  sorry
+
+lemma wX_bits_rX_bits (rs : regidx) (v : BitVec 32) :
+    (do let _ ← wX_bits rs v; rX_bits rs) =
+      (do let _ ← wX_bits rs v; pure v) := by
+  refine EStateM.ext fun reg_map => ?_
+  simp
+  rw [EStateM.run]
+  sorry
+
+lemma rX_bits_rX_bits_swap (cont : BitVec 32 → BitVec 32 → SailM α)
+    {rs rs' : regidx} (h : rs ≠ rs') :
+    (do let bv ← rX_bits rs; let bv' ← rX_bits rs'; cont bv bv') =
+      (do let bv' ← rX_bits rs'; let bv ← rX_bits rs; cont bv bv') := by
+  sorry
+
+lemma wX_bits_rX_bits_swap (cont : Unit → BitVec 32 → SailM α)
+    {rs rs' : regidx} (h : rs ≠ rs') (bv : BitVec 32) :
+    (do let u ← wX_bits rs bv; let bv' ← rX_bits rs'; cont u bv') =
+      (do let bv' ← rX_bits rs'; let _ ← wX_bits rs bv; cont () bv') := by
+  sorry
+
+lemma rX_bits_wX_bits_swap (cont : BitVec 32 → Unit → SailM α)
+    {rs rs' : regidx} (h : rs ≠ rs') (bv : BitVec 32) :
+    (do let bv ← rX_bits rs; let u ← wX_bits rs' bv; cont bv u) =
+      (do let _ ← wX_bits rs' bv; let bv ← rX_bits rs; cont bv ()) := by
+  sorry
+
+lemma wX_bits_wX_bits_swap (cont : Unit → Unit → SailM α)
+    {rs rs' : regidx} (h : rs ≠ rs') (bv bv' : BitVec 32) :
+    (do let u ← wX_bits rs bv; let u' ← wX_bits rs' bv'; cont u u') =
+      (do let _ ← wX_bits rs' bv'; let _ ← wX_bits rs bv; cont () ()) := by
+  sorry
+
+end sailboats
